Fix BabyIP example to use dependently typed syntax.

deps/poulet4/lib/P4automata/Benchmarks/BabyIP.v
@@ -1,4 +1,5 @@
 Require Coq.Classes.EquivDec.
+Require Import Coq.Arith.PeanoNat.
 Require Coq.Lists.List.
 Import List.ListNotations.
 Require Import Coq.Program.Program.
@@ -7,61 +8,39 @@ Require Import Poulet4.FinType.
 Require Import Poulet4.P4automata.Sum.
 Require Import Poulet4.P4automata.ConfRel.
 
-Ltac prep_equiv :=
-  unfold Equivalence.equiv, RelationClasses.complement in *;
-  program_simpl; try congruence.
-
-Obligation Tactic := prep_equiv.
-
 Module BabyIP1.
   Inductive state :=
   | Start
   | ParseUDP
   | ParseTCP.
+
   Scheme Equality for state.
   Global Instance state_eqdec: EquivDec.EqDec state eq := state_eq_dec.
-  Global Program Instance state_finite: @Finite state _ state_eq_dec :=
-    {| enum := [Start; ParseUDP; ParseTCP] |}.
-  Next Obligation.
-    repeat constructor;
-      repeat match goal with
-             | H: List.In _ [] |- _ => apply List.in_nil in H; exfalso; exact H
-             | |- ~ List.In _ [] => apply List.in_nil
-             | |- ~ List.In _ (_ :: _) => unfold not; intros
-             | H: List.In _ (_::_) |- _ => inversion H; clear H
-             | _ => discriminate
-             end.
-  Qed.
-  Next Obligation.
-    destruct x; intuition congruence.
+
+  Global Instance state_finite: @Finite state _ state_eq_dec.
+  Proof.
+    solve_finiteness.
   Qed.
 
-  Inductive header :=
-  | HdrIP
-  | HdrUDPTCP.
+  Inductive header : nat -> Type :=
+  | HdrIP: header 20
+  | HdrUDP: header 20
+  | HdrTCP: header 28.
 
-  Scheme Equality for header.
-  Global Instance header_eqdec: EquivDec.EqDec header eq := header_eq_dec.
-  Global Program Instance header_finite: @Finite header _ header_eq_dec :=
-    {| enum := [HdrIP; HdrUDPTCP] |}.
-  Next Obligation.
-    repeat constructor;
-      repeat match goal with
-             | H: List.In _ [] |- _ => apply List.in_nil in H; exfalso; exact H
-             | |- ~ List.In _ [] => apply List.in_nil
-             | |- ~ List.In _ (_ :: _) => unfold not; intros
-             | H: List.In _ (_::_) |- _ => inversion H; clear H
-             | _ => discriminate
-             end.
+  Global Instance header_eqdec: forall n, EquivDec.EqDec (header n) eq.
+  Proof.
+    solve_eqdec.
   Qed.
-  Next Obligation.
-    destruct x; intuition congruence.
+
+  Global Instance header_finite: forall n, @Finite (header n) _ (header_eqdec n).
+  Proof.
+    intros n; solve_indexed_finiteness n [20; 28].
   Qed.
 
   Definition states (s: state) :=
     match s with
     | Start =>
-      {| st_op := OpExtract (existT (fun _ => header) 20 HdrIP);
+      {| st_op := OpExtract (existT header 20 HdrIP);
          st_trans := P4A.TSel (CExpr (ESlice (n := 20) (EHdr HdrIP) 19 16))
                               [{| sc_pat := PExact (VBits 4 (tt, false, false, false, true));
                                   sc_st := inl ParseUDP |};
@@ -69,67 +48,49 @@ Module BabyIP1.
                                  sc_st := inl ParseTCP |}]
                               (inr false) |}
     | ParseUDP =>
-      {| st_op := OpExtract (existT _ 20 HdrUDPTCP);
+      {| st_op := OpExtract (existT header 20 HdrUDP);
          st_trans := P4A.TGoto _ (inr true) |}
     | ParseTCP =>
-      {| st_op := OpExtract (existT _ 28 HdrUDPTCP);
+      {| st_op := OpExtract (existT header 28 HdrTCP);
          st_trans := P4A.TGoto _ (inr true) |}
     end.
 
   Program Definition aut: Syntax.t state _ :=
     {| t_states := states |}.
-  Solve Obligations with (destruct s; cbv; Lia.lia).
-
+  Solve All Obligations with (destruct s; cbv; Lia.lia).
 End BabyIP1.
 
 Module BabyIP2.
   Inductive state :=
   | Start
   | ParseSeq.
+
   Scheme Equality for state.
   Global Instance state_eqdec: EquivDec.EqDec state eq := state_eq_dec.
-  Global Program Instance state_finite: @Finite state _ state_eq_dec :=
-    {| enum := [Start; ParseSeq] |}.
-  Next Obligation.
-    repeat constructor;
-      repeat match goal with
-             | H: List.In _ [] |- _ => apply List.in_nil in H; exfalso; exact H
-             | |- ~ List.In _ [] => apply List.in_nil
-             | |- ~ List.In _ (_ :: _) => unfold not; intros
-             | H: List.In _ (_::_) |- _ => inversion H; clear H
-             | _ => discriminate
-             end.
-  Qed.
-  Next Obligation.
-    destruct x; intuition congruence.
+
+  Global Instance state_finite: @Finite state _ state_eq_dec.
+  Proof.
+    solve_finiteness.
   Qed.
 
-  Inductive header :=
-  | HdrCombi
-  | HdrSeq.
+  Inductive header: nat -> Type :=
+  | HdrCombi: header 40
+  | HdrSeq: header 8.
 
-  Scheme Equality for header.
-  Global Instance header_eqdec: EquivDec.EqDec header eq := header_eq_dec.
-  Global Program Instance header_finite: @Finite header _ header_eq_dec :=
-    {| enum := [HdrCombi; HdrSeq] |}.
-  Next Obligation.
-    repeat constructor;
-      repeat match goal with
-             | H: List.In _ [] |- _ => apply List.in_nil in H; exfalso; exact H
-             | |- ~ List.In _ [] => apply List.in_nil
-             | |- ~ List.In _ (_ :: _) => unfold not; intros
-             | H: List.In _ (_::_) |- _ => inversion H; clear H
-             | _ => discriminate
-             end.
+  Global Instance header_eqdec: forall n, EquivDec.EqDec (header n) eq.
+  Proof.
+    solve_eqdec.
   Qed.
-  Next Obligation.
-    destruct x; intuition congruence.
+
+  Global Instance header_finite: forall n, @Finite (header n) _ (header_eqdec n).
+  Proof.
+    intros n; solve_indexed_finiteness n [40; 8].
   Qed.
 
   Definition states (s: state) :=
     match s with
     | Start =>
-      {| st_op := OpExtract (existT (fun _ => header) 40 HdrCombi);
+      {| st_op := OpExtract (existT header 40 HdrCombi);
          st_trans := P4A.TSel (CExpr (ESlice (n := 40) (EHdr HdrCombi) 19 16))
                               [{| sc_pat := PExact (VBits 4 (tt, false, false, false, true));
                                   sc_st := inr true |};
@@ -137,7 +98,7 @@ Module BabyIP2.
                                  sc_st := inl ParseSeq |}]
                               (inr false) |}
     | ParseSeq =>
-      {| st_op := OpExtract (existT _ 8 HdrSeq);
+      {| st_op := OpExtract (existT header 8 HdrSeq);
          st_trans := P4A.TGoto _ (inr true) |}
     end.
 
